SimplePCFa: steps and termination lemmas

proof/DDC/Language/SimplePCFa/Frame.v
@@ -1,40 +1,30 @@
 
-Require Import DDC.Language.SimplePCFa.Step.
-Require Import DDC.Language.SimplePCFa.ExpSubst.
-Require Import DDC.Language.SimplePCFa.Exp.
+Require Import DDC.Language.SimplePCFa.StepBase.
+Require Import DDC.Language.SimplePCFa.StepFrame.
 
 
-(* Frame stacks *)
-(* Holds the continuation while a 'let' expression reduces the bound term. *)
-Inductive frame : Set :=
- | F : forall (t : ty) (x : exp), frame.
-Hint Constructors frame.
-
-Definition stack := list frame.
-Hint Unfold stack.
-
-
+(******************************************************************************)
 (* Termination of an expression reduction in some context. *)
 Inductive TERMS : stack -> exp -> Prop :=
  (* A value in an empty context has terminated. *)
- | RfVal 
-   :  forall v
-   ,  TERMS nil (XVal v)
-
  | RfLetPush
-   :  forall f t1 x1 x2
-   ,  TERMS (f :> F t1 x2) x1
-   -> TERMS f (XLet t1 x1 x2)
+   :  forall fs t x1 x2
+   ,  TERMS (fs :> F t x2) x1
+   -> TERMS fs             (XLet t x1 x2)
 
  | RfLetPop
-   :  forall f t1 v1 x2
-   ,  TERMS f (substVX 0 v1 x2)
-   -> TERMS (f :> F t1 x2) (XVal v1)
+   :  forall fs t v x
+   ,  TERMS fs             (substVX 0 v x)
+   -> TERMS (fs :> F t x)  (XVal v)
 
  | RfStep
-   :  forall f x1 x1'
-   ,  STEPP x1 x1' -> TERMS f x1'
-   -> TERMS f x1.
+   :  forall fs x1 x2
+   ,  STEPP x1 x2 -> TERMS fs x2
+   -> TERMS fs x1
+
+ | RfDone
+   :  forall v
+   ,  TERMS nil (XVal v).
 Hint Constructors TERMS.
 
 
@@ -74,5 +64,168 @@ Proof.
    simpl in H. destruct a.
     lets D: IHf H.
     destruct x; inverts D; nope.
-Qed.  
+Qed.
 
+
+(******************************************************************************)
+(* Termination with STEPS *)
+Lemma steps_terms_trans
+ :  forall fs x1 x2
+ ,  TERMS fs x1
+ -> STEPS x1 x2
+ -> TERMS fs x2.
+Proof.
+ intros.
+ induction H0; eauto.
+
+  gen fs.
+  induction H0; intros; eauto.
+  destruct x1; nope.
+   inverts H0. assert (x2 = x0). admit. subst. auto.  (* determinism of STEPP *)
+   inverts H0. skip. (* determinism ok *)
+   inverts H0. skip. (* determinism ok *)
+
+   SCase "XLet".
+    eapply RfLetPush.
+    inverts H. eauto. nope.
+
+   SCase "XApp".
+    inverts H.
+    inverts H2. auto.
+    inverts H.
+    inverts H0.
+Qed.
+Hint Resolve steps_terms_trans.
+
+
+(******************************************************************************)
+(* Termination with STEPF *)
+Lemma stepf_terms
+ :  forall fs x v
+ ,  STEPF  fs x nil (XVal v)
+ -> TERMS  fs x.
+Proof.
+ intros. gen fs v. 
+ induction x; intros.
+  Case "XVal".
+   inverts H.
+    eapply RfLetPop. rs.
+    eauto.
+  Case "XLet".  nope.
+  Case "XApp".  inverts H. eauto.
+  Case "XOp1".  inverts H. eauto.
+  Case "XIf".   inverts H. eauto.
+Qed.
+
+
+Lemma stepf_terms_expand_front
+ :  forall fs1 x1 fs2 x2
+ ,  STEPF fs1 x1 fs2 x2
+ -> TERMS fs2 x2
+ -> TERMS fs1 x1.
+Proof.
+ intros fs1 x1 fs2 x2 HS HT.
+ induction HS; eauto.
+Qed.
+
+
+Lemma stepf_terms_trans
+ :  forall x1 fs1 x2 fs2
+ ,  TERMS  fs1 x1
+ -> STEPF  fs1 x1 fs2 x2
+ -> TERMS  fs2 x2.
+Proof.
+ intros.
+ induction H0; eauto.
+  (inverts H; eauto; nope).
+Qed.
+
+
+(******************************************************************************)
+(* Termination with STEPLS *)
+Lemma terms_stepls
+ :  forall fs x
+ ,  TERMS fs x
+ -> exists v, STEPLS fs x nil (XVal v).
+Proof.
+ intros.
+ induction H.
+  destruct IHTERMS as [v]. eauto.
+  destruct IHTERMS as [v0]. eauto.
+  destruct IHTERMS as [v]. eauto.
+  eauto.
+Qed.
+Hint Resolve terms_stepls.
+
+
+Lemma terms_stepls_expand_front
+ :  forall fs1 x1 fs2 x2
+ ,  STEPLS fs1 x1 fs2 x2
+ -> TERMS  fs2 x2
+ -> TERMS  fs1 x1. 
+Proof.
+ intros.
+ induction H.
+  auto.
+  eapply stepf_terms_expand_front; eauto.
+Qed.
+
+
+Lemma terms_stepls_expand_back
+ :  forall x1 fs1 x2 fs2
+ ,  STEPLS fs1 x1 fs2 x2
+ -> TERMS  fs1 x1 
+ -> TERMS  fs2 x2.
+Proof.
+ intros.
+ induction H.
+  eauto.
+  eauto using stepf_terms_trans.
+Qed.
+
+
+(******************************************************************************)
+Lemma terms_split
+ :  forall fs1 fs2 x 
+ ,  TERMS (fs1 >< fs2) x
+ -> (exists v, STEPLS fs2 x nil (XVal v)
+            /\ TERMS  fs1 (XVal v)).
+Proof.
+ intros. gen x. gen fs1.
+ induction fs2; intros.
+  Case "Nil".
+   rw (fs1 >< nil = fs1) in H.
+
+   gen x.
+   induction fs1; intros.
+    SCase "Nil".
+     lets HS: terms_stepls H. shift v. rip.
+
+    SCase "Cons".
+     destruct a.
+     lets D: RfLetPush H.
+     spec IHfs1 D.
+     destruct IHfs1 as [v]. rip.
+
+     assert (exists v1, STEPLS nil x nil (XVal v1)). 
+      admit. (* from STEPSLS, binding exp reduces to some value *)
+
+     destruct H0 as [v1].
+     exists v1. rip.
+
+     assert (STEPLS (fs1 :> F t x0) x (fs1 :> F t x0) (XVal v1)).
+      admit. (* from STEPSLS, reduction in larger stack *)
+
+     eapply terms_stepls_expand_back. eauto. eauto.
+ 
+  Case "Cons".   
+   rw (fs1 >< (fs2 :> a) = (fs1 >< fs2) :> a) in H.
+   destruct a.
+   apply RfLetPush in H.
+   lets D: IHfs2 H.
+   destruct D as [v].
+   exists v. rip.
+   inverts H1.
+   inverts H0. auto.
+   inverts H1.
+Qed.
