proof/DDC/Language/SimplePCFa/StepFrame.v
@@ -1,0 +1,60 @@
+
+Require Import DDC.Language.SimplePCFa.StepBase.
+Require Import DDC.Language.SimplePCFa.ExpSubst.
+Require Import DDC.Language.SimplePCFa.Exp.
+
+(* Frame stacks *)
+(* Holds the continuation while a 'let' expression reduces the bound term. *)
+Inductive frame : Set :=
+ | F : forall (t : ty) (x : exp), frame.
+Hint Constructors frame.
+
+Definition stack := list frame.
+Hint Unfold stack.
+
+
+(* Single step reduction under a frame stack. *)
+Inductive STEPF : stack -> exp -> stack -> exp -> Prop :=
+ | SfPush
+   :  forall fs t x1 x2
+   ,  STEPF fs             (XLet t x1 x2)
+            (fs :> F t x2) x1
+
+ | SfPop
+   :  forall fs x t v
+   ,  STEPF (fs :> F t x) (XVal v)
+            fs            (substVX 0 v x)
+
+ | SfStep
+   :  forall fs x1 x2
+   ,  STEPP x1 x2
+   -> STEPF fs x1 fs x2.
+Hint Constructors STEPF.
+
+
+(** Multi-step evaluation under a frame stack *)
+Inductive STEPLS : stack -> exp -> stack -> exp -> Prop :=
+ | SsNone
+   :  forall fs x1
+   ,  STEPLS fs x1 fs x1
+
+ | SsCons
+   :  forall fs1 x1 fs2 x2 fs3 x3
+   ,  STEPF  fs1 x1 fs2 x2 -> STEPLS fs2 x2 fs3 x3
+   -> STEPLS fs1 x1 fs3 x3.
+Hint Constructors STEPLS.
+
+
+(** Multi-step evaluation under a frame stack *)
+Inductive STEPRS : stack -> exp -> stack -> exp -> Prop :=
+ | SrNone
+   :  forall fs x1
+   ,  STEPRS fs x1 fs x1
+
+ | SrSnoc
+   :  forall fs1 x1 fs2 x2 fs3 x3
+   ,  STEPRS fs1 x1 fs2 x2 -> STEPF fs2 x2 fs3 x3 
+   -> STEPRS fs1 x1 fs3 x3.
+Hint Constructors STEPRS.
+
+
